Reconstruct blocked tasks from workload traces
Extend the Awkernel workload trace syntax and checker with Block and Unblock task events, wait classes, unblock kinds, and event ids. The common semantics remains cause-free while the adapter acceptance layer reconstructs blocked intervals and rejects blocked Choose, Dispatch, and Complete observations.

extracted/haskell/AwkernelWorkloadAcceptance.hs
@@ -208,6 +208,15 @@ data OpEvent =
  | EvStutter
  | EvTick
 
+remove_job :: JobId -> (List JobId) -> List JobId
+remove_job j xs =
+  case xs of {
+   Nil -> Nil;
+   Cons x xs' ->
+    case eqb0 x j of {
+     True -> remove_job j xs';
+     False -> Cons x (remove_job j xs')}}
+
 runs_on :: Schedule -> JobId -> Time -> CPU -> Bool
 runs_on sched j t c =
   case sched t c of {
@@ -247,39 +256,46 @@ choose_top_m g =
   g
 
 data AwkernelSchedTraceEntry =
-   MkAwkernelSchedTraceEntry CPU OpEvent (Option JobId) (List JobId) 
+   MkAwkernelSchedTraceEntry Nat CPU OpEvent (Option JobId) (List JobId) 
  Bool (Option JobId) (List (Option JobId)) (List Bool) (List (Option JobId))
+
+aste_event_id :: AwkernelSchedTraceEntry -> Nat
+aste_event_id a =
+  case a of {
+   MkAwkernelSchedTraceEntry aste_event_id0 _ _ _ _ _ _ _ _ _ ->
+    aste_event_id0}
 
 aste_cpu :: AwkernelSchedTraceEntry -> CPU
 aste_cpu a =
   case a of {
-   MkAwkernelSchedTraceEntry aste_cpu0 _ _ _ _ _ _ _ _ -> aste_cpu0}
+   MkAwkernelSchedTraceEntry _ aste_cpu0 _ _ _ _ _ _ _ _ -> aste_cpu0}
 
 aste_event :: AwkernelSchedTraceEntry -> OpEvent
 aste_event a =
   case a of {
-   MkAwkernelSchedTraceEntry _ aste_event0 _ _ _ _ _ _ _ -> aste_event0}
+   MkAwkernelSchedTraceEntry _ _ aste_event0 _ _ _ _ _ _ _ -> aste_event0}
 
 aste_current :: AwkernelSchedTraceEntry -> Option JobId
 aste_current a =
   case a of {
-   MkAwkernelSchedTraceEntry _ _ aste_current0 _ _ _ _ _ _ -> aste_current0}
+   MkAwkernelSchedTraceEntry _ _ _ aste_current0 _ _ _ _ _ _ -> aste_current0}
 
 aste_runnable :: AwkernelSchedTraceEntry -> List JobId
 aste_runnable a =
   case a of {
-   MkAwkernelSchedTraceEntry _ _ _ aste_runnable0 _ _ _ _ _ -> aste_runnable0}
+   MkAwkernelSchedTraceEntry _ _ _ _ aste_runnable0 _ _ _ _ _ ->
+    aste_runnable0}
 
 aste_need_resched :: AwkernelSchedTraceEntry -> Bool
 aste_need_resched a =
   case a of {
-   MkAwkernelSchedTraceEntry _ _ _ _ aste_need_resched0 _ _ _ _ ->
+   MkAwkernelSchedTraceEntry _ _ _ _ _ aste_need_resched0 _ _ _ _ ->
     aste_need_resched0}
 
 aste_dispatch_target :: AwkernelSchedTraceEntry -> Option JobId
 aste_dispatch_target a =
   case a of {
-   MkAwkernelSchedTraceEntry _ _ _ _ _ aste_dispatch_target0 _ _ _ ->
+   MkAwkernelSchedTraceEntry _ _ _ _ _ _ aste_dispatch_target0 _ _ _ ->
     aste_dispatch_target0}
 
 sched_trace_primary_current :: AwkernelSchedTraceEntry -> Option JobId
@@ -300,28 +316,54 @@ data AwkernelTaskTraceKind =
  | LkRunnable
  | LkChoose
  | LkDispatch
- | LkSleep
+ | LkBlock
+ | LkUnblock
  | LkJoinWait
  | LkJoinTargetReady
  | LkComplete
 
+data AwkernelWaitClass =
+   WcSleep
+ | WcIo
+
+data AwkernelUnblockKind =
+   UkReady
+ | UkTimeout
+
 data AwkernelTaskTraceEntry =
-   MkAwkernelTaskTraceEntry AwkernelTaskTraceKind JobId (Option JobId)
+   MkAwkernelTaskTraceEntry Nat AwkernelTaskTraceKind JobId (Option JobId) 
+ (Option AwkernelWaitClass) (Option AwkernelUnblockKind)
+
+atte_event_id :: AwkernelTaskTraceEntry -> Nat
+atte_event_id a =
+  case a of {
+   MkAwkernelTaskTraceEntry atte_event_id0 _ _ _ _ _ -> atte_event_id0}
 
 atte_kind :: AwkernelTaskTraceEntry -> AwkernelTaskTraceKind
 atte_kind a =
   case a of {
-   MkAwkernelTaskTraceEntry atte_kind0 _ _ -> atte_kind0}
+   MkAwkernelTaskTraceEntry _ atte_kind0 _ _ _ _ -> atte_kind0}
 
 atte_subject :: AwkernelTaskTraceEntry -> JobId
 atte_subject a =
   case a of {
-   MkAwkernelTaskTraceEntry _ atte_subject0 _ -> atte_subject0}
+   MkAwkernelTaskTraceEntry _ _ atte_subject0 _ _ _ -> atte_subject0}
 
 atte_related :: AwkernelTaskTraceEntry -> Option JobId
 atte_related a =
   case a of {
-   MkAwkernelTaskTraceEntry _ _ atte_related0 -> atte_related0}
+   MkAwkernelTaskTraceEntry _ _ _ atte_related0 _ _ -> atte_related0}
+
+atte_wait_class :: AwkernelTaskTraceEntry -> Option AwkernelWaitClass
+atte_wait_class a =
+  case a of {
+   MkAwkernelTaskTraceEntry _ _ _ _ atte_wait_class0 _ -> atte_wait_class0}
+
+atte_unblock_kind :: AwkernelTaskTraceEntry -> Option AwkernelUnblockKind
+atte_unblock_kind a =
+  case a of {
+   MkAwkernelTaskTraceEntry _ _ _ _ _ atte_unblock_kind0 ->
+    atte_unblock_kind0}
 
 option_job_eqb :: (Option JobId) -> (Option JobId) -> Bool
 option_job_eqb x y =
@@ -381,7 +423,7 @@ add_pair_once x xs =
    True -> xs;
    False -> Cons x xs}
 
-all_dependencies_ready :: JobId -> (List (Prod JobId JobId)) -> (List
+all_dependencies_ready :: JobId -> (List (Prod JobId JobId)) -> (List 
                           JobId) -> Bool
 all_dependencies_ready task_id deps ready_targets =
   case deps of {
@@ -395,16 +437,97 @@ all_dependencies_ready task_id deps ready_targets =
           (all_dependencies_ready task_id deps' ready_targets);
        False -> all_dependencies_ready task_id deps' ready_targets}}}
 
-bool_of_option_none :: (Option JobId) -> Bool
+bool_of_option_none :: (Option a1) -> Bool
 bool_of_option_none oj =
   case oj of {
    Some _ -> False;
    None -> True}
 
+bool_of_wait_class_some :: (Option AwkernelWaitClass) -> Bool
+bool_of_wait_class_some owc =
+  case owc of {
+   Some _ -> True;
+   None -> False}
+
+bool_of_unblock_kind_some :: (Option AwkernelUnblockKind) -> Bool
+bool_of_unblock_kind_some ouk =
+  case ouk of {
+   Some _ -> True;
+   None -> False}
+
+wait_class_eqb :: AwkernelWaitClass -> AwkernelWaitClass -> Bool
+wait_class_eqb lhs rhs =
+  case lhs of {
+   WcSleep -> case rhs of {
+               WcSleep -> True;
+               WcIo -> False};
+   WcIo -> case rhs of {
+            WcSleep -> False;
+            WcIo -> True}}
+
+task_trace_metadata_empty :: AwkernelTaskTraceEntry -> Bool
+task_trace_metadata_empty entry =
+  andb
+    (andb (bool_of_option_none (atte_related entry))
+      (bool_of_option_none (atte_wait_class entry)))
+    (bool_of_option_none (atte_unblock_kind entry))
+
+task_trace_has_wait_class_only :: AwkernelTaskTraceEntry -> Bool
+task_trace_has_wait_class_only entry =
+  andb
+    (andb (bool_of_option_none (atte_related entry))
+      (bool_of_wait_class_some (atte_wait_class entry)))
+    (bool_of_option_none (atte_unblock_kind entry))
+
+task_trace_has_wait_and_unblock_kind :: AwkernelTaskTraceEntry -> Bool
+task_trace_has_wait_and_unblock_kind entry =
+  andb
+    (andb (bool_of_option_none (atte_related entry))
+      (bool_of_wait_class_some (atte_wait_class entry)))
+    (bool_of_unblock_kind_some (atte_unblock_kind entry))
+
+blocked_task_class :: JobId -> (List (Prod JobId AwkernelWaitClass)) ->
+                      Option AwkernelWaitClass
+blocked_task_class task_id blocked =
+  case blocked of {
+   Nil -> None;
+   Cons p blocked' ->
+    case p of {
+     Pair blocked_task wait_class ->
+      case eqb0 blocked_task task_id of {
+       True -> Some wait_class;
+       False -> blocked_task_class task_id blocked'}}}
+
+blocked_task_contains :: JobId -> (List (Prod JobId AwkernelWaitClass)) ->
+                         Bool
+blocked_task_contains task_id blocked =
+  case blocked_task_class task_id blocked of {
+   Some _ -> True;
+   None -> False}
+
+remove_blocked_task :: JobId -> (List (Prod JobId AwkernelWaitClass)) -> List
+                       (Prod JobId AwkernelWaitClass)
+remove_blocked_task task_id blocked =
+  case blocked of {
+   Nil -> Nil;
+   Cons p blocked' ->
+    case p of {
+     Pair blocked_task wait_class ->
+      case eqb0 blocked_task task_id of {
+       True -> remove_blocked_task task_id blocked';
+       False -> Cons (Pair blocked_task wait_class)
+        (remove_blocked_task task_id blocked')}}}
+
 sched_trace_event_is_wakeup :: JobId -> AwkernelSchedTraceEntry -> Bool
 sched_trace_event_is_wakeup j entry =
   case aste_event entry of {
    EvWakeup j' -> eqb0 j' j;
+   _ -> False}
+
+sched_trace_event_is_block :: JobId -> AwkernelSchedTraceEntry -> Bool
+sched_trace_event_is_block j entry =
+  case aste_event entry of {
+   EvBlock j' -> eqb0 j' j;
    _ -> False}
 
 sched_trace_event_is_choose :: JobId -> JobId -> AwkernelSchedTraceEntry ->
@@ -451,6 +574,17 @@ sched_trace_is_wakeup j entry =
           (bool_of_option_none (sched_trace_primary_current entry)))
         (job_list_contains j (aste_runnable entry)))
       (eqb (sched_trace_primary_need_resched entry) False))
+    (bool_of_option_none (sched_trace_primary_dispatch_target entry))
+
+sched_trace_is_block :: JobId -> AwkernelSchedTraceEntry -> Bool
+sched_trace_is_block j entry =
+  andb
+    (andb
+      (andb
+        (andb (eqb0 (aste_cpu entry) (S O))
+          (sched_trace_event_is_block j entry))
+        (bool_of_option_none (sched_trace_primary_current entry)))
+      (eqb (sched_trace_primary_need_resched entry) True))
     (bool_of_option_none (sched_trace_primary_dispatch_target entry))
 
 sched_trace_is_choose :: JobId -> AwkernelSchedTraceEntry -> Bool
@@ -502,34 +636,82 @@ sched_trace_is_stutter entry =
 
 data AwkernelTaskTraceSummary =
    MkAwkernelTaskTraceSummary (Option JobId) (List JobId) (List
-                                                          (Prod JobId JobId))
- (List JobId)
+                                                          (Prod JobId JobId)) 
+ (List JobId) (List (Prod JobId AwkernelWaitClass)) (List
+                                                    (Prod Nat
+                                                    (Prod JobId Bool)))
 
 atts_root_task :: AwkernelTaskTraceSummary -> Option JobId
 atts_root_task a =
   case a of {
-   MkAwkernelTaskTraceSummary atts_root_task0 _ _ _ -> atts_root_task0}
+   MkAwkernelTaskTraceSummary atts_root_task0 _ _ _ _ _ -> atts_root_task0}
 
 atts_known_tasks :: AwkernelTaskTraceSummary -> List JobId
 atts_known_tasks a =
   case a of {
-   MkAwkernelTaskTraceSummary _ atts_known_tasks0 _ _ -> atts_known_tasks0}
+   MkAwkernelTaskTraceSummary _ atts_known_tasks0 _ _ _ _ ->
+    atts_known_tasks0}
 
 atts_completion_deps :: AwkernelTaskTraceSummary -> List (Prod JobId JobId)
 atts_completion_deps a =
   case a of {
-   MkAwkernelTaskTraceSummary _ _ atts_completion_deps0 _ ->
+   MkAwkernelTaskTraceSummary _ _ atts_completion_deps0 _ _ _ ->
     atts_completion_deps0}
 
 atts_ready_targets :: AwkernelTaskTraceSummary -> List JobId
 atts_ready_targets a =
   case a of {
-   MkAwkernelTaskTraceSummary _ _ _ atts_ready_targets0 ->
+   MkAwkernelTaskTraceSummary _ _ _ atts_ready_targets0 _ _ ->
     atts_ready_targets0}
+
+atts_blocked_tasks :: AwkernelTaskTraceSummary -> List
+                      (Prod JobId AwkernelWaitClass)
+atts_blocked_tasks a =
+  case a of {
+   MkAwkernelTaskTraceSummary _ _ _ _ atts_blocked_tasks0 _ ->
+    atts_blocked_tasks0}
+
+atts_block_transitions :: AwkernelTaskTraceSummary -> List
+                          (Prod Nat (Prod JobId Bool))
+atts_block_transitions a =
+  case a of {
+   MkAwkernelTaskTraceSummary _ _ _ _ _ atts_block_transitions0 ->
+    atts_block_transitions0}
 
 initial_task_trace_summary :: AwkernelTaskTraceSummary
 initial_task_trace_summary =
-  MkAwkernelTaskTraceSummary None Nil Nil Nil
+  MkAwkernelTaskTraceSummary None Nil Nil Nil Nil Nil
+
+add_block_transition :: Nat -> JobId -> Bool -> (List
+                        (Prod Nat (Prod JobId Bool))) -> List
+                        (Prod Nat (Prod JobId Bool))
+add_block_transition event_id task_id is_block transitions =
+  app transitions (Cons (Pair event_id (Pair task_id is_block)) Nil)
+
+task_trace_blocked_at_from :: Nat -> JobId -> (List
+                              (Prod Nat (Prod JobId Bool))) -> Bool -> Bool
+task_trace_blocked_at_from event_id task_id transitions blocked =
+  case transitions of {
+   Nil -> blocked;
+   Cons p transitions' ->
+    case p of {
+     Pair transition_event_id p0 ->
+      case p0 of {
+       Pair transition_task is_block ->
+        let {
+         blocked' = case ltb transition_event_id event_id of {
+                     True ->
+                      case eqb0 transition_task task_id of {
+                       True -> is_block;
+                       False -> blocked};
+                     False -> blocked}}
+        in
+        task_trace_blocked_at_from event_id task_id transitions' blocked'}}}
+
+task_trace_blocked_at :: AwkernelTaskTraceSummary -> Nat -> JobId -> Bool
+task_trace_blocked_at summary event_id task_id =
+  task_trace_blocked_at_from event_id task_id
+    (atts_block_transitions summary) False
 
 task_trace_entry_valid :: AwkernelTaskTraceSummary -> AwkernelTaskTraceEntry
                           -> Bool
@@ -540,25 +722,66 @@ task_trace_entry_valid summary entry =
       (negb
         (job_list_contains (atte_subject entry) (atts_known_tasks summary)))
       (case atte_related entry of {
-        Some parent -> job_list_contains parent (atts_known_tasks summary);
-        None -> option_job_eqb (atts_root_task summary) None});
+        Some parent ->
+         andb
+           (andb (job_list_contains parent (atts_known_tasks summary))
+             (bool_of_option_none (atte_wait_class entry)))
+           (bool_of_option_none (atte_unblock_kind entry));
+        None ->
+         andb
+           (andb (option_job_eqb (atts_root_task summary) None)
+             (bool_of_option_none (atte_wait_class entry)))
+           (bool_of_option_none (atte_unblock_kind entry))});
+   LkBlock ->
+    andb
+      (andb
+        (job_list_contains (atte_subject entry) (atts_known_tasks summary))
+        (negb
+          (blocked_task_contains (atte_subject entry)
+            (atts_blocked_tasks summary))))
+      (task_trace_has_wait_class_only entry);
+   LkUnblock ->
+    andb
+      (andb
+        (job_list_contains (atte_subject entry) (atts_known_tasks summary))
+        (task_trace_has_wait_and_unblock_kind entry))
+      (case atte_wait_class entry of {
+        Some wait_class ->
+         case blocked_task_class (atte_subject entry)
+                (atts_blocked_tasks summary) of {
+          Some blocked_wait_class ->
+           wait_class_eqb wait_class blocked_wait_class;
+          None -> False};
+        None -> False});
    LkJoinWait ->
     case atte_related entry of {
      Some target ->
       andb
-        (job_list_contains (atte_subject entry) (atts_known_tasks summary))
-        (job_list_contains target (atts_known_tasks summary));
+        (andb
+          (andb
+            (job_list_contains (atte_subject entry)
+              (atts_known_tasks summary))
+            (job_list_contains target (atts_known_tasks summary)))
+          (bool_of_option_none (atte_wait_class entry)))
+        (bool_of_option_none (atte_unblock_kind entry));
      None -> False};
    LkJoinTargetReady ->
     case atte_related entry of {
      Some _ -> False;
      None ->
       andb
-        (job_list_contains (atte_subject entry) (atts_known_tasks summary))
-        (negb
-          (job_list_contains (atte_subject entry)
-            (atts_ready_targets summary)))};
-   _ -> job_list_contains (atte_subject entry) (atts_known_tasks summary)}
+        (andb
+          (andb
+            (job_list_contains (atte_subject entry)
+              (atts_known_tasks summary))
+            (negb
+              (job_list_contains (atte_subject entry)
+                (atts_ready_targets summary))))
+          (bool_of_option_none (atte_wait_class entry)))
+        (bool_of_option_none (atte_unblock_kind entry))};
+   _ ->
+    andb (job_list_contains (atte_subject entry) (atts_known_tasks summary))
+      (task_trace_metadata_empty entry)}
 
 task_trace_entry_step :: AwkernelTaskTraceSummary -> AwkernelTaskTraceEntry
                          -> AwkernelTaskTraceSummary
@@ -569,18 +792,36 @@ task_trace_entry_step summary entry =
       Some _ -> atts_root_task summary;
       None -> Some (atte_subject entry)})
     (add_job_once (atte_subject entry) (atts_known_tasks summary))
-    (atts_completion_deps summary) (atts_ready_targets summary);
+    (atts_completion_deps summary) (atts_ready_targets summary)
+    (atts_blocked_tasks summary) (atts_block_transitions summary);
+   LkBlock -> MkAwkernelTaskTraceSummary (atts_root_task summary)
+    (atts_known_tasks summary) (atts_completion_deps summary)
+    (atts_ready_targets summary) (Cons (Pair (atte_subject entry)
+    (case atte_wait_class entry of {
+      Some wait_class -> wait_class;
+      None -> WcSleep}))
+    (atts_blocked_tasks summary))
+    (add_block_transition (atte_event_id entry) (atte_subject entry) True
+      (atts_block_transitions summary));
+   LkUnblock -> MkAwkernelTaskTraceSummary (atts_root_task summary)
+    (atts_known_tasks summary) (atts_completion_deps summary)
+    (atts_ready_targets summary)
+    (remove_blocked_task (atte_subject entry) (atts_blocked_tasks summary))
+    (add_block_transition (atte_event_id entry) (atte_subject entry) False
+      (atts_block_transitions summary));
    LkJoinWait ->
     case atte_related entry of {
      Some target -> MkAwkernelTaskTraceSummary (atts_root_task summary)
       (atts_known_tasks summary)
       (add_pair_once (Pair (atte_subject entry) target)
         (atts_completion_deps summary))
-      (atts_ready_targets summary);
+      (atts_ready_targets summary) (atts_blocked_tasks summary)
+      (atts_block_transitions summary);
      None -> summary};
    LkJoinTargetReady -> MkAwkernelTaskTraceSummary (atts_root_task summary)
     (atts_known_tasks summary) (atts_completion_deps summary)
-    (add_job_once (atte_subject entry) (atts_ready_targets summary));
+    (add_job_once (atte_subject entry) (atts_ready_targets summary))
+    (atts_blocked_tasks summary) (atts_block_transitions summary);
    _ -> summary}
 
 summarize_task_trace :: AwkernelTaskTraceSummary -> (List
@@ -597,41 +838,47 @@ summarize_task_trace summary task_trace =
 
 data AwkernelSchedTraceAcceptanceState =
    MkAwkernelSchedTraceAcceptanceState Bool (Option JobId) (List JobId) 
- (List JobId) (List JobId)
+ (List JobId) (List JobId) (List JobId)
 
 astas_started :: AwkernelSchedTraceAcceptanceState -> Bool
 astas_started a =
   case a of {
-   MkAwkernelSchedTraceAcceptanceState astas_started0 _ _ _ _ ->
+   MkAwkernelSchedTraceAcceptanceState astas_started0 _ _ _ _ _ ->
     astas_started0}
 
 astas_selected :: AwkernelSchedTraceAcceptanceState -> Option JobId
 astas_selected a =
   case a of {
-   MkAwkernelSchedTraceAcceptanceState _ astas_selected0 _ _ _ ->
+   MkAwkernelSchedTraceAcceptanceState _ astas_selected0 _ _ _ _ ->
     astas_selected0}
 
 astas_dispatched :: AwkernelSchedTraceAcceptanceState -> List JobId
 astas_dispatched a =
   case a of {
-   MkAwkernelSchedTraceAcceptanceState _ _ astas_dispatched0 _ _ ->
+   MkAwkernelSchedTraceAcceptanceState _ _ astas_dispatched0 _ _ _ ->
     astas_dispatched0}
 
 astas_completed :: AwkernelSchedTraceAcceptanceState -> List JobId
 astas_completed a =
   case a of {
-   MkAwkernelSchedTraceAcceptanceState _ _ _ astas_completed0 _ ->
+   MkAwkernelSchedTraceAcceptanceState _ _ _ astas_completed0 _ _ ->
     astas_completed0}
 
 astas_ready_targets :: AwkernelSchedTraceAcceptanceState -> List JobId
 astas_ready_targets a =
   case a of {
-   MkAwkernelSchedTraceAcceptanceState _ _ _ _ astas_ready_targets0 ->
+   MkAwkernelSchedTraceAcceptanceState _ _ _ _ astas_ready_targets0 _ ->
     astas_ready_targets0}
+
+astas_blocked :: AwkernelSchedTraceAcceptanceState -> List JobId
+astas_blocked a =
+  case a of {
+   MkAwkernelSchedTraceAcceptanceState _ _ _ _ _ astas_blocked0 ->
+    astas_blocked0}
 
 initial_sched_trace_acceptance_state :: AwkernelSchedTraceAcceptanceState
 initial_sched_trace_acceptance_state =
-  MkAwkernelSchedTraceAcceptanceState False None Nil Nil Nil
+  MkAwkernelSchedTraceAcceptanceState False None Nil Nil Nil Nil
 
 sched_trace_step_start :: AwkernelTaskTraceSummary -> AwkernelSchedTraceEntry
                           -> Option AwkernelSchedTraceAcceptanceState
@@ -639,7 +886,8 @@ sched_trace_step_start summary entry =
   case atts_root_task summary of {
    Some root ->
     case sched_trace_is_wakeup root entry of {
-     True -> Some (MkAwkernelSchedTraceAcceptanceState True None Nil Nil Nil);
+     True -> Some (MkAwkernelSchedTraceAcceptanceState True None Nil Nil Nil
+      Nil);
      False -> None};
    None -> None}
 
@@ -656,28 +904,52 @@ sched_trace_step_after_start summary st entry =
     case andb
            (andb (sched_trace_is_wakeup j entry) (job_list_contains j known))
            (negb (job_list_contains j (astas_completed st))) of {
-     True -> Some st;
+     True -> Some (MkAwkernelSchedTraceAcceptanceState True
+      (astas_selected st) (astas_dispatched st) (astas_completed st)
+      (astas_ready_targets st) (remove_job j (astas_blocked st)));
+     False -> None}}
+  in
+  let {
+   try_block_job = \j ->
+    case andb
+           (andb
+             (andb (sched_trace_is_block j entry)
+               (job_list_contains j known))
+             (negb (job_list_contains j (astas_completed st))))
+           (negb (job_list_contains j (astas_blocked st))) of {
+     True -> Some (MkAwkernelSchedTraceAcceptanceState True None
+      (astas_dispatched st) (astas_completed st) (astas_ready_targets st)
+      (add_job_once j (astas_blocked st)));
      False -> None}}
   in
   let {
    try_choose_job = \j ->
     case andb
            (andb
-             (andb (sched_trace_is_choose j entry)
-               (job_list_contains j known))
-             (negb (job_list_contains j (astas_completed st))))
+             (andb
+               (andb
+                 (andb (sched_trace_is_choose j entry)
+                   (job_list_contains j known))
+                 (negb (job_list_contains j (astas_completed st))))
+               (negb (job_list_contains j (astas_blocked st))))
+             (negb (task_trace_blocked_at summary (aste_event_id entry) j)))
            (option_job_eqb (astas_selected st) None) of {
      True -> Some (MkAwkernelSchedTraceAcceptanceState True (Some j)
-      (astas_dispatched st) (astas_completed st) (astas_ready_targets st));
+      (astas_dispatched st) (astas_completed st) (astas_ready_targets st)
+      (astas_blocked st));
      False -> None}}
   in
   let {
    try_dispatch_job = \j ->
-    case andb (sched_trace_is_dispatch j entry)
-           (option_job_eqb (astas_selected st) (Some j)) of {
+    case andb
+           (andb
+             (andb (sched_trace_is_dispatch j entry)
+               (option_job_eqb (astas_selected st) (Some j)))
+             (negb (job_list_contains j (astas_blocked st))))
+           (negb (task_trace_blocked_at summary (aste_event_id entry) j)) of {
      True -> Some (MkAwkernelSchedTraceAcceptanceState True None
       (add_job_once j (astas_dispatched st)) (astas_completed st)
-      (astas_ready_targets st));
+      (astas_ready_targets st) (astas_blocked st));
      False -> None}}
   in
   let {
@@ -690,20 +962,24 @@ sched_trace_step_after_start summary st entry =
            (negb (job_list_contains j (astas_ready_targets st))) of {
      True -> Some (MkAwkernelSchedTraceAcceptanceState True None
       (astas_dispatched st) (astas_completed st)
-      (add_job_once j (astas_ready_targets st)));
+      (add_job_once j (astas_ready_targets st)) (astas_blocked st));
      False -> None}}
   in
   let {
    try_complete_job = \j ->
     case andb
            (andb
-             (andb (sched_trace_is_complete j entry)
-               (job_list_contains j (astas_dispatched st)))
-             (negb (job_list_contains j (astas_completed st))))
+             (andb
+               (andb
+                 (andb (sched_trace_is_complete j entry)
+                   (job_list_contains j (astas_dispatched st)))
+                 (negb (job_list_contains j (astas_completed st))))
+               (negb (job_list_contains j (astas_blocked st))))
+             (negb (task_trace_blocked_at summary (aste_event_id entry) j)))
            (all_dependencies_ready j deps (astas_ready_targets st)) of {
      True -> Some (MkAwkernelSchedTraceAcceptanceState True None
       (astas_dispatched st) (add_job_once j (astas_completed st))
-      (astas_ready_targets st));
+      (astas_ready_targets st) (astas_blocked st));
      False -> None}}
   in
   case sched_trace_is_stutter entry of {
@@ -712,15 +988,18 @@ sched_trace_step_after_start summary st entry =
     case first_some try_wakeup_job known of {
      Some st' -> Some st';
      None ->
-      case first_some try_choose_job known of {
+      case first_some try_block_job known of {
        Some st' -> Some st';
        None ->
-        case first_some try_dispatch_job known of {
+        case first_some try_choose_job known of {
          Some st' -> Some st';
          None ->
-          case first_some try_join_target_ready known of {
+          case first_some try_dispatch_job known of {
            Some st' -> Some st';
-           None -> first_some try_complete_job known}}}}}
+           None ->
+            case first_some try_join_target_ready known of {
+             Some st' -> Some st';
+             None -> first_some try_complete_job known}}}}}}
 
 sched_trace_step :: AwkernelTaskTraceSummary ->
                     AwkernelSchedTraceAcceptanceState ->
@@ -779,7 +1058,7 @@ row_candidate_visibleb row j =
 
 empty_sched_trace_entry :: AwkernelSchedTraceEntry
 empty_sched_trace_entry =
-  MkAwkernelSchedTraceEntry O EvStutter None Nil False None Nil Nil Nil
+  MkAwkernelSchedTraceEntry O O EvStutter None Nil False None Nil Nil Nil
 
 fifo_eligible_candidates :: (JobId -> Job) -> Nat -> Schedule -> Time ->
                             (List JobId) -> List JobId
@@ -1074,3 +1353,4 @@ awk_workload_accepts_global_fifo_scheduler_relation_sched_trace task_trace sched
   andb (awk_workload_accepts_sched_trace task_trace sched_trace)
     (sched_trace_global_fifo_scheduler_relation_checkb task_trace
       sched_trace)
+
